bug with universes :-(

theories/test_param.v
@@ -3,7 +3,6 @@ Cd "~/git/coq-elpi".
 
 From elpi Require Import elpi.
 
-Set Printing Universes.
 Class param_db {X X1 XR : Type} (x : X) (x : X1) (xR : XR) := store_param {}.
 Class param {X : Type} {XR : X -> X -> Type} (x : X) (xR : XR x x) := Param {}.
 
@@ -18,8 +17,79 @@ Elpi Print param "param.html"
   "lp-lib.elpi"
   "coq-refiner.elpi".
 
-Elpi Run param "env-add-param {{@unit}} ""unitR""".
-Elpi Run param "env-add-param {{@nat}} ""natR""".
+
+Set Printing Universes.
+(* Elpi Run param "env-add-param {{@nat}} ""natR""". *)
+Inductive natR : nat -> nat -> Set :=
+    natR_O : natR 0 0
+  | natR_S : (fun f g : nat -> nat => forall H H0 : nat, natR H H0 -> natR (f H) (g H0)) S S.
+Instance: param_db nat nat natR.
+Instance: param_db O O natR_O.
+Instance: param_db S S natR_S.
+
+Inductive vec (A : Type) : nat -> Type :=
+    nil : vec A 0 | cons : A -> forall n : nat, vec A n -> vec A (S n).
+(* Elpi Run param "env-add-param {{@vec}} ""vecR"")". *)
+Inductive
+vecR (A A0 : Type) (A1 : A -> A0 -> Type) : forall H H0 : nat, natR H H0 -> vec A H -> vec A0 H0 -> Type :=
+    vecR_nil : vecR A A0 A1 0 0 natR_O (nil A) (nil A0)
+  | vecR_cons : forall (H : A) (H0 : A0),
+                A1 H H0 ->
+                forall (n n0 : nat) (n1 : natR n n0) (H1 : vec A n) (H2 : vec A0 n0),
+                vecR A A0 A1 n n0 n1 H1 H2 ->
+                vecR A A0 A1 (S n) (S n0) (natR_S n n0 n1) (cons A H n H1) (cons A0 H0 n0 H2).
+Instance: param_db vec vec vecR.
+Instance: param_db nil nil vecR_nil.
+Instance: param_db cons cons vecR_cons.
+
+Definition vec_length_type := forall (A : Type) (n : nat), vec A n -> nat.
+Fail Elpi Run param "env-add-param {{@vec_length_type}} ""vec_length_typeR"")".
+
+Definition vec_length_typeR : (forall (A : Type) (n : nat), vec A n -> nat) ->
+       (forall (A : Type) (n : nat), vec A n -> nat) -> Type :=
+fun f g : forall (A : Type) (n : nat), vec A n -> nat =>
+forall (A A0 : Type) (A1 : A -> A0 -> Type) (n n0 : nat) (n1 : natR n n0) (H : vec A n) (H0 : vec A0 n0),
+vecR A A0 A1 n n0 n1 H H0 -> natR (f A n H) (g A0 n0 H0).
+Instance: param_db vec_length_type vec_length_type vec_length_typeR.
+
+Definition vec_length_rec (vec_length : vec_length_type)
+  (A : Type) n (v : vec A n) :=
+  match v with nil _ => 0 | cons _ _ _ w => S (vec_length _ _ w) end.
+Elpi Run param "env-add-param {{@vec_length_rec}} ""vec_length_recR"")".
+
+Elpi Run param "param-const {{@vec_length_rec}} _ _ _ _ XR TR".
+
+(* Elpi Run param " *)
+(*      coq-env-const {term->gr {{@vec_length_rec}}} X _, *)
+(*      with-TC-param (param X X1 XR), *)
+(*      coq-elaborate X X' T', *)
+(*      coq-elaborate X1 X1' T1', *)
+(*      coq-elaborate XR XR' TR', *)
+(*      coq-env-add-const ""vec_length_recR'"" XR' TR' _)". *)
+
+Definition vec_length_recR' :=
+fun (vec_length vec_length0 : vec_length_type) (vec_length1 : vec_length_typeR vec_length vec_length0)
+  (A A0 : Type) (A1 : A -> A0 -> Type) (n n0 : nat) (n1 : natR n n0) (v : vec A n) 
+  (v0 : vec A0 n0) (v1 : vecR A A0 A1 n n0 n1 v v0) =>
+match
+  v1 in (vecR _ _ _ n2 n3 n4 v2 v3)
+  return
+    (natR match v2 with
+          | nil _ => 0
+          | cons _ _ n5 w => S (vec_length A n5 w)
+          end match v3 with
+              | nil _ => 0
+              | cons _ _ n5 w => S (vec_length0 A0 n5 w)
+              end)
+with
+| vecR_nil _ _ _ => natR_O
+| vecR_cons _ _ _ _ _ _ n2 n3 n4 w w0 w1 =>
+    natR_S (vec_length A n2 w) (vec_length0 A0 n3 w0) (vec_length1 A A0 A1 n2 n3 n4 w w0 w1)
+end.
+
+Fail Elpi Run param "env-add-param {{@vec_length_rec}} ""vec_length_recR"")".
+
+(* Definition vec_length_recR := vec_length_recR'. *)
 
 Inductive fin : nat -> Type :=
     FO : fin 0 | FS : forall n : nat, fin n -> fin (S n).
@@ -28,10 +98,6 @@ Elpi Run param "env-add-param {{@fin}} ""finR"")".
 Fixpoint fin_length  n (v : fin n) :=
   match v with FO => 0 | FS _ w => S (fin_length _ w) end.
 Elpi Run param "env-add-param {{@fin_length}} ""fin_lengthR"")".
-
-Inductive vec (A : Type) : nat -> Type :=
-    nil : vec A 0 | cons : A -> forall n : nat, vec A n -> vec A (S n).
-Elpi Run param "env-add-param {{@vec}} ""vecR"")".
 
 Fixpoint vec_length (A : Type) n (v : vec A n) :=
   match v with nil _ => 0 | cons _ _ _ w => S (vec_length _ _ w) end.
@@ -64,13 +130,6 @@ Elpi Run param "env-add-param {{@test}} ""testR""".
 (*   Z = X, TZ = TX. *)
 (* ". *)
 
-Definition vec_length_type := forall (A : Type) (n : nat), vec A n -> nat.
-Elpi Run param "env-add-param {{@vec_length_type}} ""vec_length_typeR"")".
-
-Definition vec_length_rec (vec_length : vec_length_type)
-  (A : Type) n (v : vec A n) :=
-  match v with nil _ => 0 | cons _ _ _ w => S (vec_length _ _ w) end.
-Elpi Run param "env-add-param {{@vec_length_rec}} ""vec_length_recR"")".
 
 
 Elpi Run param "with-TC-param (param {{O}} X Y)".
